Add files via upload

nGerman.thy
@@ -28,7 +28,7 @@ definition n_RecvGntE :: "nat \<Rightarrow> rule" where
     assign (Para ''Cache.State'' i, Const E) ||
     assign (Para ''Chan2.Cmd'' i, Const Empty)"
 
-lemma RecvGntE:
+lemma symRecvGntE:
   "symParamRule N n_RecvGntE"
   "wellFormedStatement N (act (n_RecvGntE i))"
   "absTransfRule M (n_RecvGntE i) = (if i \<le> M then n_RecvGntE i else chaos \<triangleright> skip)"
@@ -41,7 +41,7 @@ definition n_RecvGntS :: "nat \<Rightarrow> rule" where
     assign (Para ''Cache.State'' i, Const S) ||
     assign (Para ''Chan2.Cmd'' i, Const Empty)"
 
-lemma RecvGntS:
+lemma symRecvGntS:
   "symParamRule N n_RecvGntS"
   "wellFormedStatement N (act (n_RecvGntS i))"
   "absTransfRule M (n_RecvGntS i) = (if i \<le> M then n_RecvGntS i else chaos \<triangleright> skip)"
@@ -70,7 +70,7 @@ definition n_SendGntE_abs :: "nat \<Rightarrow> rule" where
     assign (Ident ''ExGntd'', Const true) ||
     assign (Ident ''CurCmd'', Const Empty)"
 
-lemma wellFormedSendGntE:
+lemma symSendGntE:
   "symParamRule N (n_SendGntE N)"
   "wellFormedStatement N (act (n_SendGntE N i))"
   unfolding n_SendGntE_def
@@ -101,7 +101,7 @@ definition n_SendGntS_abs :: "nat \<Rightarrow> rule" where
    \<triangleright>
     assign (Ident ''CurCmd'', Const Empty)"
 
-lemma wellFormedSendGntS:
+lemma symSendGntS:
   "symParamRule N n_SendGntS"
   "wellFormedStatement N (act (n_SendGntS i))"
   unfolding n_SendGntS_def
@@ -129,7 +129,7 @@ definition n_RecvInvAck1_abs :: rule where
    \<triangleright>
     assign (Ident ''ExGntd'', Const false)"
 
-lemma RecvInvAck1:
+lemma symRecvInvAck1:
   "symParamRule N n_RecvInvAck1"
   "wellFormedStatement N (act (n_RecvInvAck1 i))"
   "absTransfRule M (n_RecvInvAck1 i) = (if i \<le> M then n_RecvInvAck1 i else n_RecvInvAck1_abs)"
@@ -151,7 +151,7 @@ definition n_RecvInvAck2_abs :: rule where
    \<triangleright>
     skip"
 
-lemma RecvInvAck2:
+lemma symRecvInvAck2:
   "symParamRule N n_RecvInvAck2"
   "wellFormedStatement N (act (n_RecvInvAck2 i))"
   "absTransfRule M (n_RecvInvAck2 i) = (if i \<le> M then n_RecvInvAck2 i else n_RecvInvAck2_abs)"
@@ -167,7 +167,7 @@ definition n_SendInvAck1 :: "nat \<Rightarrow> rule" where
     assign (Para ''Chan3.Cmd'' i, Const InvAck) ||
     assign (Para ''Cache.State'' i, Const I)"
 
-lemma SendInvAck1:
+lemma symSendInvAck1:
   "symParamRule N n_SendInvAck1"
   "wellFormedStatement N (act (n_SendInvAck1 i))"
   "absTransfRule M (n_SendInvAck1 i) = (if i \<le> M then n_SendInvAck1 i else chaos \<triangleright> skip)"
@@ -183,7 +183,7 @@ definition n_SendInvAck2 :: "nat \<Rightarrow> rule" where
     assign (Para ''Chan3.Cmd'' i, Const InvAck) ||
     assign (Para ''Cache.State'' i, Const I)"
 
-lemma SendInvAck2:
+lemma symSendInvAck2:
   "symParamRule N n_SendInvAck2"
   "wellFormedStatement N (act (n_SendInvAck2 i))"
   "absTransfRule M (n_SendInvAck2 i) = (if i \<le> M then n_SendInvAck2 i else chaos \<triangleright> skip)"
@@ -204,7 +204,7 @@ definition n_SendInv1_abs :: rule where
    \<triangleright>
     skip"
 
-lemma SendInv1:
+lemma symSendInv1:
   "symParamRule N n_SendInv1"
   "wellFormedStatement N (act (n_SendInv1 i))"
   "absTransfRule M (n_SendInv1 i) = (if i \<le> M then n_SendInv1 i else n_SendInv1_abs)"
@@ -227,7 +227,7 @@ definition n_SendInv2_abs :: rule where
    \<triangleright>
     skip"
 
-lemma SendInv2:
+lemma symSendInv2:
   "symParamRule N n_SendInv2"
   "wellFormedStatement N (act (n_SendInv2 i))"
   "absTransfRule M (n_SendInv2 i) = (if i \<le> M then n_SendInv2 i else n_SendInv2_abs)"
@@ -251,7 +251,7 @@ definition n_RecvReqE_abs :: "nat \<Rightarrow> rule" where
     assign (Ident ''CurPtr'', Const (index (M+1))) ||
     forallStm (\<lambda>j. assign (Para ''InvSet'' j, IVar (Para ''ShrSet'' j))) M"
 
-lemma wellFormedReqE:
+lemma symRecvReqE:
   "symParamRule N (n_RecvReqE N)"
   "wellFormedStatement N (act (n_RecvReqE N i))"
   unfolding n_RecvReqE_def
@@ -280,7 +280,7 @@ definition n_RecvReqS_abs :: "nat \<Rightarrow> rule" where
     assign (Ident ''CurPtr'', Const (index (M+1))) ||
     forallStm (\<lambda>j. assign (Para ''InvSet'' j, IVar (Para ''ShrSet'' j))) M"
 
-lemma wellFormedRecvReqS:
+lemma symRecvReqS:
   "symParamRule N (n_RecvReqS N)"
   "wellFormedStatement N (act (n_RecvReqS N i))"
   unfolding n_RecvReqS_def
@@ -299,7 +299,7 @@ definition n_SendReqE1 :: "nat \<Rightarrow> rule" where
    \<triangleright>
     assign (Para ''Chan1.Cmd'' i, Const ReqE)"
 
-lemma SendReqE1:
+lemma symSendReqE1:
   "symParamRule N n_SendReqE1"
   "wellFormedStatement N (act (n_SendReqE1 i))"
   "absTransfRule M (n_SendReqE1 i) = (if i \<le> M then n_SendReqE1 i else chaos \<triangleright> skip)"
@@ -312,7 +312,7 @@ definition n_SendReqE2 :: "nat \<Rightarrow> rule" where
    \<triangleright>
     assign (Para ''Chan1.Cmd'' i, Const ReqE)"
 
-lemma SendReqE2:
+lemma symSendReqE2:
   "symParamRule N n_SendReqE2"
   "wellFormedStatement N (act (n_SendReqE2 i))"
   "absTransfRule M (n_SendReqE2 i) = (if i \<le> M then n_SendReqE2 i else chaos \<triangleright> skip)"
@@ -349,29 +349,158 @@ definition rules :: "nat \<Rightarrow> rule set" where
     (\<exists>i. i\<le>N \<and> r=n_SendReqE2 i) \<or>
     (\<exists>i. i\<le>N \<and> r=n_SendReqS i)
   }"
+definition n_RecvGntEs::" nat\<Rightarrow>rule set" where  
+  "n_RecvGntEs N== oneParamCons N  n_RecvGntE"
 
-definition initSpec0 :: "nat \<Rightarrow> formula" where
+definition n_RecvGntSs::" nat\<Rightarrow>rule set" where 
+  "n_RecvGntSs N== oneParamCons N  n_RecvGntS"
+
+definition n_SendGntEs::" nat\<Rightarrow>rule set" where  
+  "n_SendGntEs N== oneParamCons N  (n_SendGntE N)"
+
+definition n_SendGntSs::" nat\<Rightarrow>rule set" where  
+  "n_SendGntSs N== oneParamCons N  n_SendGntS"
+
+definition n_RecvInvAck1s::" nat\<Rightarrow>rule set" where  
+  "n_RecvInvAck1s N== oneParamCons N  n_RecvInvAck1"
+
+definition n_RecvInvAck2s::" nat\<Rightarrow>rule set" where 
+  "n_RecvInvAck2s N== oneParamCons N  n_RecvInvAck2"
+
+definition n_SendInvAck1s::" nat\<Rightarrow>rule set" where  
+  "n_SendInvAck1s N== oneParamCons N  (n_SendInvAck1 )"
+
+definition n_SendInvAck2s::" nat\<Rightarrow>rule set" where  
+  "n_SendInvAck2s N== oneParamCons N  (n_SendInvAck2 )"
+
+definition n_SendInv1s::" nat\<Rightarrow>rule set" where  
+  "n_SendInv1s N== oneParamCons N n_SendInv1"
+
+definition n_SendInv2s::" nat\<Rightarrow>rule set" where  
+  "n_SendInv2s N== oneParamCons N  (n_SendInv2 )"
+
+definition n_RecvReqEs::" nat\<Rightarrow>rule set" where  
+  "n_RecvReqEs N== oneParamCons N  (n_RecvReqE N )"
+
+definition n_RecvReqSs::" nat\<Rightarrow>rule set" where  
+  "n_RecvReqSs N== oneParamCons N (n_RecvReqS N)"
+
+definition n_SendReqE1s::" nat\<Rightarrow>rule set" where  
+  "n_SendReqE1s N== oneParamCons N n_SendReqE1"
+
+definition n_SendReqE2s::" nat\<Rightarrow>rule set" where  
+  "n_SendReqE2s N== oneParamCons N  n_SendReqE2 "
+
+definition n_SendReqSs::" nat\<Rightarrow>rule set" where  
+  "n_SendReqSs N== oneParamCons N  (n_SendReqS )"
+
+ 
+definition rules' :: "nat \<Rightarrow> rule set" where [simp]:
+  "rules' N \<equiv>  (n_RecvGntEs N) \<union>
+    (n_RecvGntSs N) \<union>
+    (n_SendGntEs  N) \<union>
+    (n_SendGntSs N) \<union>
+    ( n_RecvInvAck1s N)\<union>
+    ( n_RecvInvAck2s N) \<union>
+    ( n_SendInvAck1s N) \<union>
+    ( n_SendInvAck2s N) \<union>
+    ( n_SendInv1s N) \<union>
+    ( n_SendInv2s N) \<union>
+    ( n_RecvReqEs  N) \<union>
+    ( n_RecvReqSs  N) \<union>
+    ( n_SendReqE1s N) \<union>
+    ( n_SendReqE2s N) \<union>
+    ( n_SendReqSs N) 
+   "
+lemma n_RecvGntEsIsSym:
+  "symProtRules' N (n_RecvGntEs N)"
+  using symRecvGntE(1) n_RecvGntEs_def symParaRuleInfSymRuleSet by auto
+
+lemma n_RecvGntSsIsSym:
+  "symProtRules' N (n_RecvGntSs N)"
+  using n_RecvGntSs_def symRecvGntS(1) symParaRuleInfSymRuleSet by auto 
+
+lemma n_SendGntEsIsSym:
+  "symProtRules' N (n_SendGntEs N)"
+  using n_SendGntEs_def symSendGntE(1) symParaRuleInfSymRuleSet by auto 
+
+lemma n_SendGntSsIsSym:
+  "symProtRules' N (n_SendGntSs N)"  
+  using n_SendGntSs_def symSendGntS(1) symParaRuleInfSymRuleSet by auto
+
+lemma  n_RecvInvAck1sIsSym:
+  "symProtRules' N ( n_RecvInvAck1s N)"
+  using symRecvInvAck1(1)  n_RecvInvAck1s_def symParaRuleInfSymRuleSet by auto
+
+lemma n_RecvInvAck2sIsSym:
+  "symProtRules' N (n_RecvInvAck2s N)"
+  using n_RecvInvAck2s_def symRecvInvAck2(1) symParaRuleInfSymRuleSet by auto 
+
+lemma n_SendInvAck1sIsSym:
+  "symProtRules' N (n_SendInvAck1s N)"
+  using n_SendInvAck1s_def symSendInvAck1(1) symParaRuleInfSymRuleSet by auto 
+
+lemma n_SendInvAck2sIsSym:
+  "symProtRules' N (n_SendInvAck2s N)"
+  using n_SendInvAck2s_def symSendInvAck2(1) symParaRuleInfSymRuleSet by auto 
+
+lemma n_SendInv1sIsSym:
+  "symProtRules' N (n_SendInv1s N)"
+  using n_SendInv1s_def symSendInv1(1) symParaRuleInfSymRuleSet by auto 
+
+lemma n_SendInv2sIsSym:
+  "symProtRules' N (n_SendInv2s N)"
+  using n_SendInv2s_def symSendInv2(1) symParaRuleInfSymRuleSet by auto 
+
+lemma n_RecvReqEsIsSym:
+  "symProtRules' N (n_RecvReqEs N)"
+  using n_RecvReqEs_def symRecvReqE(1) symParaRuleInfSymRuleSet by auto 
+
+lemma n_RecvReqSsIsSym:
+  "symProtRules' N (n_RecvReqSs N)"
+  using n_RecvReqSs_def symRecvReqS(1) symParaRuleInfSymRuleSet by auto 
+
+lemma n_SendReqE1sIsSym:
+  "symProtRules' N (n_SendReqE1s N)"
+  using n_SendReqE1s_def symSendReqE1(1) symParaRuleInfSymRuleSet by auto 
+
+lemma n_SendReqE2sIsSym:
+  "symProtRules' N (n_SendReqE2s N)"
+  using n_SendReqE2s_def symSendReqE2(1) symParaRuleInfSymRuleSet by auto 
+
+lemma n_SendReqSsIsSym:
+  "symProtRules' N (n_SendReqSs N)"
+  using n_SendReqSs_def symSendReqS(1) symParaRuleInfSymRuleSet by auto
+ 
+
+lemma rulesSym':
+  shows "symProtRules' N (rules' N)"
+  using n_RecvGntEsIsSym n_RecvGntSsIsSym n_RecvInvAck1sIsSym n_RecvInvAck2sIsSym n_RecvReqEsIsSym n_RecvReqSsIsSym n_SendGntEsIsSym n_SendGntSsIsSym n_SendInv1sIsSym n_SendInv2sIsSym n_SendInvAck1sIsSym n_SendInvAck2sIsSym n_SendReqE1sIsSym 
+n_SendReqE2sIsSym n_SendReqSsIsSym rules'_def symProtRulesUnion by presburger 
+ 
+
+definition initSpec0 :: "nat \<Rightarrow> formula" where [simp]:
   "initSpec0 N \<equiv> (\<forall>\<^sub>fi. IVar (Para ''Chan1.Cmd'' i) =\<^sub>f Const Empty) N"
 
-definition initSpec1 :: "nat \<Rightarrow> formula" where
+definition initSpec1 :: "nat \<Rightarrow> formula" where [simp]:
   "initSpec1 N \<equiv> (\<forall>\<^sub>fi. IVar (Para ''Chan2.Cmd'' i) =\<^sub>f Const Empty) N"
 
-definition initSpec2 :: "nat \<Rightarrow> formula" where
+definition initSpec2 :: "nat \<Rightarrow> formula" where [simp]:
   "initSpec2 N \<equiv> (\<forall>\<^sub>fi. IVar (Para ''Chan3.Cmd'' i) =\<^sub>f Const Empty) N"
 
-definition initSpec3 :: "nat \<Rightarrow> formula" where
+definition initSpec3 :: "nat \<Rightarrow> formula" where [simp]:
   "initSpec3 N \<equiv> (\<forall>\<^sub>fi. IVar (Para ''Cache.State'' i) =\<^sub>f Const I) N"
 
-definition initSpec4 :: "nat \<Rightarrow> formula" where
+definition initSpec4 :: "nat \<Rightarrow> formula" where [simp]:
   "initSpec4 N \<equiv> (\<forall>\<^sub>fi. IVar (Para ''InvSet'' i) =\<^sub>f Const false) N"
 
-definition initSpec5 :: "nat \<Rightarrow> formula" where
+definition initSpec5 :: "nat \<Rightarrow> formula" where [simp]:
   "initSpec5 N \<equiv> (\<forall>\<^sub>fi. IVar (Para ''ShrSet'' i) =\<^sub>f Const false) N"
 
-definition initSpec6 :: formula where
+definition initSpec6 :: formula where [simp]:
   "initSpec6 \<equiv> IVar (Ident ''ExGntd'') =\<^sub>f Const false"
 
-definition initSpec7 :: formula where
+definition initSpec7 :: formula where [simp]:
   "initSpec7 \<equiv> IVar (Ident ''CurCmd'') =\<^sub>f Const Empty"
 
 lemma absInitSpec:
@@ -400,44 +529,54 @@ definition allInitSpecs :: "nat \<Rightarrow> formula list" where
     initSpec7
   ]"
 
-definition invAux :: "nat \<Rightarrow> nat \<Rightarrow> formula" where
+definition invAux :: "nat \<Rightarrow> nat \<Rightarrow> formula" where  
   "invAux N i \<equiv>
      IVar (Para ''Chan3.Cmd'' i) =\<^sub>f Const InvAck \<and>\<^sub>f
      \<not>\<^sub>f IVar (Ident ''CurCmd'') =\<^sub>f Const Empty \<and>\<^sub>f
      IVar (Ident ''ExGntd'') =\<^sub>f Const true \<longrightarrow>\<^sub>f
-     forallFormExcl (\<lambda>j. \<not>\<^sub>f IVar (Para ''Cache.State'' j) =\<^sub>f Const E) i N \<and>\<^sub>f
+    forallFormExcl 
+    (\<lambda>j. ((\<not>\<^sub>f (IVar (Para ''Cache.State'' j) =\<^sub>f Const E))  \<and>\<^sub>f
+       ( \<not>\<^sub>f (IVar (Para ''Chan2.Cmd'' j) =\<^sub>f Const GntE))  \<and>\<^sub>f
+       ( \<not>\<^sub>f (IVar (Para ''Chan3.Cmd'' j) =\<^sub>f Const InvAck))
+    )) i N"
+     (*forallFormExcl (\<lambda>j. \<not>\<^sub>f IVar (Para ''Cache.State'' j) =\<^sub>f Const E) i N \<and>\<^sub>f
      forallFormExcl (\<lambda>j. \<not>\<^sub>f IVar (Para ''Chan2.Cmd'' j) =\<^sub>f Const GntE) i N \<and>\<^sub>f
-     forallFormExcl (\<lambda>j. \<not>\<^sub>f IVar (Para ''Chan3.Cmd'' j) =\<^sub>f Const InvAck) i N"
+     forallFormExcl (\<lambda>j. \<not>\<^sub>f IVar (Para ''Chan3.Cmd'' j) =\<^sub>f Const InvAck) i N"*)
 
-definition n_RecvInvAck1' :: "nat \<Rightarrow> nat \<Rightarrow> rule" where
+definition n_RecvInvAck1' :: "nat \<Rightarrow> nat \<Rightarrow> rule" where  
   "n_RecvInvAck1' N i = strengthenRule2 (invAux N i) (n_RecvInvAck1 i)"
 
-definition n_RecvInvAck1'_ref :: "nat \<Rightarrow> nat \<Rightarrow> rule" where
+definition n_RecvInvAck1'_ref :: "nat \<Rightarrow> nat \<Rightarrow> rule" where 
   "n_RecvInvAck1'_ref N i \<equiv>
     (IVar (Para ''Chan3.Cmd'' i) =\<^sub>f Const InvAck \<and>\<^sub>f
      \<not>\<^sub>f IVar (Ident ''CurCmd'') =\<^sub>f Const Empty \<and>\<^sub>f
      IVar (Ident ''ExGntd'') =\<^sub>f Const true) \<and>\<^sub>f
-    forallFormExcl (\<lambda>j. \<not>\<^sub>f IVar (Para ''Cache.State'' j) =\<^sub>f Const E) i N \<and>\<^sub>f
-    forallFormExcl (\<lambda>j. \<not>\<^sub>f IVar (Para ''Chan2.Cmd'' j) =\<^sub>f Const GntE) i N \<and>\<^sub>f
-    forallFormExcl (\<lambda>j. \<not>\<^sub>f IVar (Para ''Chan3.Cmd'' j) =\<^sub>f Const InvAck) i N
+   forallFormExcl 
+    (\<lambda>j. ((\<not>\<^sub>f (IVar (Para ''Cache.State'' j) =\<^sub>f Const E))  \<and>\<^sub>f
+       ( \<not>\<^sub>f (IVar (Para ''Chan2.Cmd'' j) =\<^sub>f Const GntE))  \<and>\<^sub>f
+       ( \<not>\<^sub>f (IVar (Para ''Chan3.Cmd'' j) =\<^sub>f Const InvAck))
+    )) i N
    \<triangleright>
     assign (Para ''Chan3.Cmd'' i, Const Empty) ||
     assign (Para ''ShrSet'' i, Const false) ||
     assign (Ident ''ExGntd'', Const false)"
 
-definition n_RecvInvAck1'_abs :: "nat \<Rightarrow> rule" where
+definition n_RecvInvAck1'_abs :: "nat \<Rightarrow> rule" where   
   "n_RecvInvAck1'_abs M \<equiv>
     (\<not>\<^sub>f IVar (Ident ''CurCmd'') =\<^sub>f Const Empty \<and>\<^sub>f
      IVar (Ident ''ExGntd'') =\<^sub>f Const true) \<and>\<^sub>f
-    forallForm (\<lambda>j. \<not>\<^sub>f IVar (Para ''Cache.State'' j) =\<^sub>f Const E) M \<and>\<^sub>f
-    forallForm (\<lambda>j. \<not>\<^sub>f IVar (Para ''Chan2.Cmd'' j) =\<^sub>f Const GntE) M \<and>\<^sub>f
-    forallForm (\<lambda>j. \<not>\<^sub>f IVar (Para ''Chan3.Cmd'' j) =\<^sub>f Const InvAck) M
+    forallForm(\<lambda>j. ((\<not>\<^sub>f (IVar (Para ''Cache.State'' j) =\<^sub>f Const E))  \<and>\<^sub>f
+       ( \<not>\<^sub>f (IVar (Para ''Chan2.Cmd'' j) =\<^sub>f Const GntE))  \<and>\<^sub>f
+       ( \<not>\<^sub>f (IVar (Para ''Chan3.Cmd'' j) =\<^sub>f Const InvAck))
+    )) M  
    \<triangleright>
     assign (Ident ''ExGntd'', Const false)"
 
-lemma n_RecvInvAck1'Eq:
+(*lemma n_RecvInvAck1'Eq:
   "n_RecvInvAck1' N i = n_RecvInvAck1'_ref N i"
-  by (auto simp add: n_RecvInvAck1'_def invAux_def n_RecvInvAck1_def n_RecvInvAck1'_ref_def)
+  apply (auto simp add: n_RecvInvAck1'_def invAux_def n_RecvInvAck1_def 
+      n_RecvInvAck1'_ref_def )
+  sorry*)
 
 lemma wellFormedSendReqE2:
   "symParamRule N (n_RecvInvAck1'_ref N)"
@@ -451,4 +590,1032 @@ lemma absRecvInvAck1'b:
     (if i \<le> M then n_RecvInvAck1 i else n_RecvInvAck1'_abs M)"
   unfolding n_RecvInvAck1_def n_RecvInvAck1'_ref_def n_RecvInvAck1'_abs_def by auto
 
+
+definition pair1:: "((nat\<Rightarrow>formula)\<times>(nat\<Rightarrow>formula))" where [simp]:
+ "pair1 ==(%i. IVar (Para ''Chan3.Cmd'' i) =\<^sub>f Const InvAck \<and>\<^sub>f
+     \<not>\<^sub>f IVar (Ident ''CurCmd'') =\<^sub>f Const Empty \<and>\<^sub>f
+     IVar (Ident ''ExGntd'') =\<^sub>f Const true  ,
+                  (\<lambda>j. ((\<not>\<^sub>f (IVar (Para ''Cache.State'' j) =\<^sub>f Const E))  \<and>\<^sub>f
+       ( \<not>\<^sub>f (IVar (Para ''Chan2.Cmd'' j) =\<^sub>f Const GntE))  \<and>\<^sub>f
+       ( \<not>\<^sub>f (IVar (Para ''Chan3.Cmd'' j) =\<^sub>f Const InvAck))))
+    ) "
+
+definition F::"((nat\<Rightarrow>formula)\<times>(nat\<Rightarrow>formula)) set" where  
+"F \<equiv> {pair1}"
+
+  
+definition n_RecvInvAck12s::" nat \<Rightarrow>rule set" where 
+  "n_RecvInvAck12s N==
+  (oneParamCons N  (%i. (strengthenRule2  (constrInvByExcl pair1 i N) (n_RecvInvAck1 i))))"
+
+  
+definition rules2' :: "nat \<Rightarrow> rule set" where [simp]:
+  "rules2' N \<equiv>  (n_RecvGntEs N) \<union>
+    (n_RecvGntSs N) \<union>
+    (n_SendGntEs  N) \<union>
+    (n_SendGntSs N) \<union>
+    ( n_RecvInvAck12s N)\<union>
+    ( n_RecvInvAck2s N) \<union>
+    ( n_SendInvAck1s N) \<union>
+    ( n_SendInvAck2s N) \<union>
+    ( n_SendInv1s N) \<union>
+    ( n_SendInv2s N) \<union>
+    ( n_RecvReqEs  N) \<union>
+    ( n_RecvReqSs  N) \<union>
+    ( n_SendReqE1s N) \<union>
+    ( n_SendReqE2s N) \<union>
+    ( n_SendReqSs N)  
+    "
+
+
+definition absRules' :: " nat\<Rightarrow>rule set" where [simp]:
+  
+  "absRules' M \<equiv> (n_RecvGntEs M) \<union>
+    (n_RecvGntSs M) \<union>
+    (n_SendGntEs  M) \<union>
+    (n_SendGntSs M) \<union>
+    ( n_RecvInvAck1s M)\<union>
+    ( n_RecvInvAck2s M) \<union>
+    ( n_SendInvAck1s M) \<union>
+    ( n_SendInvAck2s M) \<union>
+    ( n_SendInv1s M) \<union>
+    ( n_SendInv2s M) \<union>
+    ( n_RecvReqEs  M) \<union>
+    ( n_RecvReqSs  M) \<union>
+    ( n_SendReqE1s M) \<union>
+    ( n_SendReqE2s M) \<union>
+    ( n_SendReqSs M) \<union>
+    {  n_SendGntE_abs M}\<union>
+    {n_SendGntS_abs M} \<union> 
+    {n_RecvInvAck1'_abs M }\<union> 
+    {n_RecvInvAck2_abs }\<union>
+    { n_SendInv1_abs}\<union>
+    { n_SendInv2_abs}\<union>
+    {n_RecvReqE_abs M}\<union>
+    {n_RecvReqS_abs M}\<union>
+    {chaos \<triangleright> skip}
+    "
+
+ 
+
+   
+
+lemma absRecvGntEs:
+  "M < N \<Longrightarrow> absTransfRule M ` (n_RecvGntEs N) = (n_RecvGntEs M) \<union> {chaos \<triangleright> skip}"
+  unfolding n_RecvGntEs_def apply (rule absGen) 
+  using symRecvGntE(3) apply blast
+  by simp  
+
+lemma absRecvGntSs:
+  "M < N \<Longrightarrow> absTransfRule M ` (n_RecvGntSs N) = (n_RecvGntSs M) \<union> {chaos \<triangleright> skip}"
+  unfolding n_RecvGntSs_def apply (rule absGen) 
+  using symRecvGntS(3) apply blast
+  by simp 
+
+lemma absSendGntEs:
+  "M < N \<Longrightarrow> absTransfRule M ` (n_SendGntEs N) = (n_SendGntEs M) \<union> {n_SendGntE_abs M}"
+  unfolding n_SendGntEs_def apply (rule absGen) thm absSendGntE
+  using absSendGntE apply auto[1]
+    by (simp  )
+
+lemma absSendGntSs:
+  "M < N \<Longrightarrow> absTransfRule M ` (n_SendGntSs N) = (n_SendGntSs M) \<union> {n_SendGntS_abs M}"
+  unfolding n_SendGntSs_def apply (rule absGen) thm absSendGntS
+  using absSendGntS apply blast
+    by (simp  )
+   
+
+lemma absRecvInvAck2s:
+  "M < N \<Longrightarrow> absTransfRule M ` (n_RecvInvAck2s N) = (n_RecvInvAck2s M) \<union> {n_RecvInvAck2_abs }"
+  unfolding n_RecvInvAck2s_def apply (rule absGen)
+  using symRecvInvAck2(3) apply blast
+  by simp  
+
+lemma n_RecvInvAck12_ref':
+  "strengthenRule2 (constrInvByExcl pair1 i N) (n_RecvInvAck1 i) = n_RecvInvAck1'_ref N i"
+  unfolding n_RecvInvAck1'_ref_def n_RecvInvAck1_def constrInvByExcl_def pair1_def fst_conv snd_conv
+  by (auto simp add: strengthenRule2.simps)
+ 
+lemma absRecvInvAck1s:
+  "M < N \<Longrightarrow> absTransfRule M ` (n_RecvInvAck12s N) = (n_RecvInvAck1s M) \<union> {n_RecvInvAck1'_abs M}"
+  unfolding n_RecvInvAck12s_def n_RecvInvAck1s_def apply (rule absGen)
+  using absRecvInvAck1'b n_RecvInvAck12_ref' apply auto[1]
+  by simp
+
+lemma absSendInvAck1s:
+  "M < N \<Longrightarrow> absTransfRule M ` (n_SendInvAck1s N) = (n_SendInvAck1s M) \<union> {chaos \<triangleright> skip}"
+  unfolding n_SendInvAck1s_def  apply (rule absGen)
+  using symSendInvAck1(3) apply blast
+  by simp 
+
+lemma absSendInvAck2s:
+  "M < N \<Longrightarrow> absTransfRule M ` (n_SendInvAck2s N) = (n_SendInvAck2s M) \<union> {chaos \<triangleright> skip}"
+  unfolding n_SendInvAck2s_def  apply (rule absGen)
+  using symSendInvAck2(3) apply blast
+  by simp 
+
+lemma absSendInv1s:
+  "M < N \<Longrightarrow> absTransfRule M ` (n_SendInv1s N) = (n_SendInv1s M) \<union> {n_SendInv1_abs}"
+  unfolding n_SendInv1s_def  apply (rule absGen)
+  using symSendInv1(3) apply blast
+  by simp 
+ 
+lemma absSendInv2s:
+  "M < N \<Longrightarrow> absTransfRule M ` (n_SendInv2s N) = (n_SendInv2s M) \<union> {n_SendInv2_abs}"
+  unfolding n_SendInv2s_def  apply (rule absGen)
+  using symSendInv2(3) apply blast
+  by simp  
+
+lemma absRecvReqEs:
+  "M < N \<Longrightarrow> absTransfRule M ` (n_RecvReqEs N) = (n_RecvReqEs M) \<union> {n_RecvReqE_abs M}"
+  unfolding n_RecvReqEs_def  apply (rule absGen)
+  using absRecvReqE apply blast 
+  by simp
+
+lemma absRecvReqSs:
+  "M < N \<Longrightarrow> absTransfRule M ` (n_RecvReqSs N) = (n_RecvReqSs M) \<union> {n_RecvReqS_abs M}"
+  unfolding n_RecvReqSs_def  apply (rule absGen)
+  using absRecvReqS apply blast 
+  by simp
+
+lemma absSendReqE1s:
+  "M < N \<Longrightarrow> absTransfRule M ` (n_SendReqE1s N) = (n_SendReqE1s M) \<union> {chaos \<triangleright> skip}"
+  unfolding n_SendReqE1s_def  apply (rule absGen)
+  using symSendReqE1(3) apply blast 
+  by simp 
+
+lemma absSendReqE2s:
+  "M < N \<Longrightarrow> absTransfRule M ` (n_SendReqE2s N) = (n_SendReqE2s M) \<union> {chaos \<triangleright> skip}"
+  unfolding n_SendReqE2s_def  apply (rule absGen)
+  using symSendReqE2(3) apply blast 
+  by simp
+
+lemma absSendReqSs:
+  "M < N \<Longrightarrow> absTransfRule M ` (n_SendReqSs N) = (n_SendReqSs M) \<union> {chaos \<triangleright> skip}"
+  unfolding n_SendReqSs_def  apply (rule absGen)
+  using symSendReqS(3) apply blast 
+  by simp
+thm strengthenRule2.simps 
+ 
+definition absRules :: "nat \<Rightarrow> rule set" where
+  "absRules N \<equiv> (n_RecvGntEs N) \<union>
+    (n_RecvGntSs N) \<union>
+    (n_SendGntEs  N) \<union>
+    (n_SendGntSs N) \<union>
+    ( n_RecvInvAck1s N)\<union>
+    ( n_RecvInvAck2s N) \<union>
+    ( n_SendInvAck1s N) \<union>
+    ( n_SendInvAck2s N) \<union>
+    ( n_SendInv1s N) \<union>
+    ( n_SendInv2s N) \<union>
+    ( n_RecvReqEs  N) \<union>
+    ( n_RecvReqSs  N) \<union>
+    ( n_SendReqE1s N) \<union>
+    ( n_SendReqE2s N) \<union>
+    ( n_SendReqSs N)\<union>{  n_SendGntE_abs N}\<union>
+    {n_SendGntS_abs N} \<union> 
+    {n_RecvInvAck1'_abs N}\<union> 
+    {n_RecvInvAck2_abs }\<union>
+    { n_SendInv1_abs}\<union>
+    { n_SendInv2_abs}\<union>
+    {n_RecvReqE_abs N}\<union>
+    {n_RecvReqS_abs N}\<union>
+    {chaos \<triangleright> skip}
+    "
+
+lemma absAll:
+  "M < N \<Longrightarrow> absTransfRule M ` rules2' N = absRules M"
+  unfolding rules2'_def absRules_def absRules_def image_Un 
+    absRecvGntEs
+    absRecvGntSs
+    absSendGntEs
+    absSendGntSs
+    absRecvInvAck1s
+    absRecvInvAck2s
+    absSendInvAck1s
+    absSendInvAck2s
+    absSendInv1s
+    absSendInv2s
+    absRecvReqEs
+    absRecvReqSs
+    absSendReqE1s
+    absSendReqE2s
+    absSendReqSs by auto
+
+lemma symPreds0[intro]:
+  "symPredSet' N ({(initSpec0 N)} )"
+unfolding initSpec0_def
+    apply (rule symPredSetForall)
+  unfolding symParamForm_def by auto 
+
+lemma symPreds1[intro]:
+  "symPredSet' N ({(initSpec1 N)} )"
+unfolding initSpec1_def
+    apply (rule symPredSetForall)
+  unfolding symParamForm_def by auto
+
+lemma symPreds2[intro]:
+  "symPredSet' N ({(initSpec2 N)} )"
+unfolding initSpec2_def
+    apply (rule symPredSetForall)
+  unfolding symParamForm_def by auto 
+
+lemma symPreds3[intro]:
+  "symPredSet' N ({(initSpec3 N)} )"
+unfolding initSpec3_def
+    apply (rule symPredSetForall)
+  unfolding symParamForm_def by auto 
+
+lemma symPreds4[intro]:
+  "symPredSet' N ({(initSpec4 N)} )"
+unfolding initSpec4_def
+    apply (rule symPredSetForall)
+  unfolding symParamForm_def by auto 
+
+lemma symPreds5[intro]:
+  "symPredSet' N ({(initSpec5 N)} )"
+unfolding initSpec5_def
+    apply (rule symPredSetForall)
+  unfolding symParamForm_def by auto 
+
+lemma symPreds6[intro]:
+  "symPredSet' N ({(initSpec6 )} )"
+  unfolding symPredSet'_def initSpec6_def by auto
+
+lemma symPreds7[intro]:
+  "symPredSet' N ({(initSpec7 )} )"
+  unfolding symPredSet'_def initSpec7_def by auto
+
+lemma symPreds:
+  "symPredSet' N ({(initSpec0 N)} \<union>
+    {(initSpec1 N)}\<union>
+    {(initSpec2 N)}\<union>
+    {(initSpec3 N)}\<union>
+    {(initSpec4 N)}\<union>
+    {(initSpec5 N)}\<union>
+    {initSpec6} \<union>
+    {initSpec7})"
+  
+  apply (meson symPreds0 symPreds1 symPreds2 symPreds3 symPreds4 symPreds5 symPreds6 symPreds7 symPredsUnion)
+   
+  done 
+
+definition type_inv_Chan3_Cmd :: "nat \<Rightarrow> state \<Rightarrow> bool" where
+  "type_inv_Chan3_Cmd N s = 
+(\<forall>i. i \<le> N \<longrightarrow> s (Para ''Chan3.Cmd'' i) = InvAck \<or> s (Para ''Chan3.Cmd'' i) = Empty)
+ "
+
+lemma n_RecvGntE_type_inv_Chan3_Cmd [intro]:
+  "type_inv_Chan3_Cmd N sk \<Longrightarrow> i \<le> N \<Longrightarrow> type_inv_Chan3_Cmd N (trans1 (act (n_RecvGntE i)) sk)"
+  unfolding type_inv_Chan3_Cmd_def n_RecvGntE_def by auto
+
+lemma n_RecvGntS_type_inv_Chan3_Cmd [intro]:
+  "type_inv_Chan3_Cmd N sk \<Longrightarrow> i \<le> N \<Longrightarrow> type_inv_Chan3_Cmd N (trans1 (act (n_RecvGntS i)) sk)"
+  unfolding type_inv_Chan3_Cmd_def n_RecvGntS_def by auto
+
+
+lemma n_SendGntE_type_inv_Chan3_Cmd [intro]:
+  "type_inv_Chan3_Cmd N sk \<Longrightarrow> i \<le> N \<Longrightarrow> type_inv_Chan3_Cmd N (trans1 (act (n_SendGntE N i)) sk)"
+  unfolding type_inv_Chan3_Cmd_def n_SendGntE_def by auto
+
+lemma n_SendGntS_type_inv_Chan3_Cmd [intro]:
+  "type_inv_Chan3_Cmd N sk \<Longrightarrow> i \<le> N \<Longrightarrow> type_inv_Chan3_Cmd N (trans1 (act (n_SendGntS  i)) sk)"
+  unfolding type_inv_Chan3_Cmd_def n_SendGntS_def by auto
+
+lemma n_RecvInvAck12_type_inv_Chan3_Cmd [intro]:
+  "type_inv_Chan3_Cmd N sk \<Longrightarrow> i \<le> N \<Longrightarrow> 
+  type_inv_Chan3_Cmd N 
+  (trans1 (act ( (strengthenRule2  (constrInvByExcl pair1 i N) (n_RecvInvAck1 i)))) sk)"
+  unfolding type_inv_Chan3_Cmd_def n_RecvInvAck1_def apply (auto simp add:strengthenRule2.simps )
+  done
+
+lemma n_RecvInvAck2_type_inv_Chan3_Cmd [intro]:
+  "type_inv_Chan3_Cmd N sk \<Longrightarrow> i \<le> N \<Longrightarrow> 
+  type_inv_Chan3_Cmd N 
+  (trans1 (act (  (n_RecvInvAck2 i))) sk)"
+  unfolding type_inv_Chan3_Cmd_def n_RecvInvAck2_def apply (auto simp add:strengthenRule2.simps )
+  done
+lemma n_SendInvAck1_type_inv_Chan3_Cmd [intro]:
+  "type_inv_Chan3_Cmd N sk \<Longrightarrow> i \<le> N \<Longrightarrow> type_inv_Chan3_Cmd N (trans1 (act (n_SendInvAck1 i)) sk)"
+  unfolding type_inv_Chan3_Cmd_def n_SendInvAck1_def by auto
+
+lemma n_SendInvAck2_type_inv_Chan3_Cmd [intro]:
+  "type_inv_Chan3_Cmd N sk \<Longrightarrow> i \<le> N \<Longrightarrow> type_inv_Chan3_Cmd N (trans1 (act (n_SendInvAck2 i)) sk)"
+  unfolding type_inv_Chan3_Cmd_def n_SendInvAck2_def by auto
+
+lemma n_SendInv1_type_inv_Chan3_Cmd [intro]:
+  "type_inv_Chan3_Cmd N sk \<Longrightarrow> i \<le> N \<Longrightarrow> type_inv_Chan3_Cmd N (trans1 (act (n_SendInv1 i)) sk)"
+  unfolding type_inv_Chan3_Cmd_def n_SendInv1_def by auto
+
+lemma n_SendInv2_type_inv_Chan3_Cmd [intro]:
+  "type_inv_Chan3_Cmd N sk \<Longrightarrow> i \<le> N \<Longrightarrow> type_inv_Chan3_Cmd N (trans1 (act (n_SendInv2 i)) sk)"
+  unfolding type_inv_Chan3_Cmd_def n_SendInv2_def by auto
+
+
+lemma n_RecvReqE_type_inv_Chan3_Cmd [intro]:
+  "type_inv_Chan3_Cmd N sk \<Longrightarrow> i \<le> N \<Longrightarrow> type_inv_Chan3_Cmd N (trans1 (act (n_RecvReqE N i)) sk)"
+  unfolding type_inv_Chan3_Cmd_def n_RecvReqE_def by auto 
+
+lemma n_RecvReqS_type_inv_Chan3_Cmd [intro]:
+  "type_inv_Chan3_Cmd N sk \<Longrightarrow> i \<le> N \<Longrightarrow> type_inv_Chan3_Cmd N (trans1 (act (n_RecvReqS N i)) sk)"
+  unfolding type_inv_Chan3_Cmd_def n_RecvReqS_def by auto
+
+lemma n_SendReqE1_type_inv_Chan3_Cmd [intro]:
+  "type_inv_Chan3_Cmd N sk \<Longrightarrow> i \<le> N \<Longrightarrow> type_inv_Chan3_Cmd N (trans1 (act (n_SendReqE1  i)) sk)"
+  unfolding type_inv_Chan3_Cmd_def n_SendReqE1_def by auto
+
+lemma n_SendReqE2_type_inv_Chan3_Cmd [intro]:
+  "type_inv_Chan3_Cmd N sk \<Longrightarrow> i \<le> N \<Longrightarrow> type_inv_Chan3_Cmd N (trans1 (act (n_SendReqE2  i)) sk)"
+  unfolding type_inv_Chan3_Cmd_def n_SendReqE2_def by auto
+
+lemma n_SendReqS_type_inv_Chan3_Cmd [intro]:
+  "type_inv_Chan3_Cmd N sk \<Longrightarrow> i \<le> N \<Longrightarrow> type_inv_Chan3_Cmd N (trans1 (act (n_SendReqS  i)) sk)"
+  unfolding type_inv_Chan3_Cmd_def n_SendReqS_def by auto 
+
+
+lemma inv_Chan3_Cmd' [simp,intro]:
+  assumes "reachableUpTo (set (allInitSpecs N)) (rules2' N) k s"
+  shows "type_inv_Chan3_Cmd N s"
+  apply (rule invIntro[OF _ _ assms])
+  subgoal for s
+    by (auto simp add: type_inv_Chan3_Cmd_def allInitSpecs_def )
+  subgoal for r sk
+    unfolding rules2'_def apply (auto simp add: pair1_def)
+    subgoal unfolding n_RecvGntEs_def  by auto
+    subgoal unfolding n_RecvGntSs_def   by auto
+    subgoal unfolding  n_SendGntEs_def by auto 
+    subgoal unfolding  n_SendGntSs_def by auto  
+    subgoal unfolding   n_RecvInvAck12s_def
+      using n_RecvInvAck12_type_inv_Chan3_Cmd by auto  
+    subgoal
+      using   n_RecvInvAck2s_def by auto
+    subgoal
+      using  n_SendInvAck1s_def by auto  
+    subgoal
+      using n_SendInvAck2s_def by auto 
+    subgoal
+      using  n_SendInv1s_def by auto  
+    subgoal
+      using n_SendInv2s_def by auto 
+    subgoal
+      using  n_RecvReqEs_def by auto  
+    subgoal
+      using n_RecvReqSs_def by auto 
+    subgoal
+      using n_SendReqE1s_def by auto 
+    subgoal
+      using n_SendReqE2s_def by auto  
+    subgoal
+      using n_SendReqSs_def by auto 
+
+    
+    done
+  done
+   
+
+lemma inv_Chan3_Cmd'' [simp,intro]:
+  assumes a: "reachableUpTo fs rs k s"
+  shows "fs =(set (allInitSpecs N))  \<longrightarrow> rs = rules2' N \<longrightarrow> i \<le> N \<longrightarrow> isEnumVal s (Para ''Chan3.Cmd'' i)"
+  using inv_Chan3_Cmd' unfolding type_inv_Chan3_Cmd_def InvAck_def InvAck_def
+  by (metis Empty_def assms getValueType.simps(1) isEnumVal_def typeOf_def)   
+
+ 
+
+definition type_inv_Chan2_Cmd :: "nat \<Rightarrow> state \<Rightarrow> bool" where
+  "type_inv_Chan2_Cmd N s = 
+(\<forall>i. i \<le> N \<longrightarrow> s (Para ''Chan2.Cmd'' i) = GntS \<or> s (Para ''Chan2.Cmd'' i) = GntE \<or>
+s (Para ''Chan2.Cmd'' i) = Inv \<or>
+s (Para ''Chan2.Cmd'' i) = Empty)
+ "
+
+lemma n_RecvGntE_type_inv_Chan2_Cmd [intro]:
+  "type_inv_Chan2_Cmd N sk \<Longrightarrow> i \<le> N \<Longrightarrow> type_inv_Chan2_Cmd N (trans1 (act (n_RecvGntE i)) sk)"
+  unfolding type_inv_Chan2_Cmd_def n_RecvGntE_def by auto
+
+lemma n_RecvGntS_type_inv_Chan2_Cmd [intro]:
+  "type_inv_Chan2_Cmd N sk \<Longrightarrow> i \<le> N \<Longrightarrow> type_inv_Chan2_Cmd N (trans1 (act (n_RecvGntS i)) sk)"
+  unfolding type_inv_Chan2_Cmd_def n_RecvGntS_def by auto
+
+
+lemma n_SendGntE_type_inv_Chan2_Cmd [intro]:
+  "type_inv_Chan2_Cmd N sk \<Longrightarrow> i \<le> N \<Longrightarrow> type_inv_Chan2_Cmd N (trans1 (act (n_SendGntE N i)) sk)"
+  unfolding type_inv_Chan2_Cmd_def n_SendGntE_def by auto
+
+lemma n_SendGntS_type_inv_Chan2_Cmd [intro]:
+  "type_inv_Chan2_Cmd N sk \<Longrightarrow> i \<le> N \<Longrightarrow> type_inv_Chan2_Cmd N (trans1 (act (n_SendGntS  i)) sk)"
+  unfolding type_inv_Chan2_Cmd_def n_SendGntS_def by auto
+
+lemma n_RecvInvAck12_type_inv_Chan2_Cmd [intro]:
+  "type_inv_Chan2_Cmd N sk \<Longrightarrow> i \<le> N \<Longrightarrow> 
+  type_inv_Chan2_Cmd N 
+  (trans1 (act ( (strengthenRule2  (constrInvByExcl pair1 i N) (n_RecvInvAck1 i)))) sk)"
+  unfolding type_inv_Chan2_Cmd_def n_RecvInvAck1_def apply (auto simp add:strengthenRule2.simps )
+  done
+
+lemma n_RecvInvAck2_type_inv_Chan2_Cmd [intro]:
+  "type_inv_Chan2_Cmd N sk \<Longrightarrow> i \<le> N \<Longrightarrow> 
+  type_inv_Chan2_Cmd N 
+  (trans1 (act (  (n_RecvInvAck2 i))) sk)"
+  unfolding type_inv_Chan2_Cmd_def n_RecvInvAck2_def apply (auto simp add:strengthenRule2.simps )
+  done
+lemma n_SendInvAck1_type_inv_Chan2_Cmd [intro]:
+  "type_inv_Chan2_Cmd N sk \<Longrightarrow> i \<le> N \<Longrightarrow> type_inv_Chan2_Cmd N (trans1 (act (n_SendInvAck1 i)) sk)"
+  unfolding type_inv_Chan2_Cmd_def n_SendInvAck1_def by auto
+
+lemma n_SendInvAck2_type_inv_Chan2_Cmd [intro]:
+  "type_inv_Chan2_Cmd N sk \<Longrightarrow> i \<le> N \<Longrightarrow> type_inv_Chan2_Cmd N (trans1 (act (n_SendInvAck2 i)) sk)"
+  unfolding type_inv_Chan2_Cmd_def n_SendInvAck2_def by auto
+
+lemma n_SendInv1_type_inv_Chan2_Cmd [intro]:
+  "type_inv_Chan2_Cmd N sk \<Longrightarrow> i \<le> N \<Longrightarrow> type_inv_Chan2_Cmd N (trans1 (act (n_SendInv1 i)) sk)"
+  unfolding type_inv_Chan2_Cmd_def n_SendInv1_def by auto
+
+lemma n_SendInv2_type_inv_Chan2_Cmd [intro]:
+  "type_inv_Chan2_Cmd N sk \<Longrightarrow> i \<le> N \<Longrightarrow> type_inv_Chan2_Cmd N (trans1 (act (n_SendInv2 i)) sk)"
+  unfolding type_inv_Chan2_Cmd_def n_SendInv2_def by auto
+
+
+lemma n_RecvReqE_type_inv_Chan2_Cmd [intro]:
+  "type_inv_Chan2_Cmd N sk \<Longrightarrow> i \<le> N \<Longrightarrow> type_inv_Chan2_Cmd N (trans1 (act (n_RecvReqE N i)) sk)"
+  unfolding type_inv_Chan2_Cmd_def n_RecvReqE_def by auto 
+
+lemma n_RecvReqS_type_inv_Chan2_Cmd [intro]:
+  "type_inv_Chan2_Cmd N sk \<Longrightarrow> i \<le> N \<Longrightarrow> type_inv_Chan2_Cmd N (trans1 (act (n_RecvReqS N i)) sk)"
+  unfolding type_inv_Chan2_Cmd_def n_RecvReqS_def by auto
+
+lemma n_SendReqE1_type_inv_Chan2_Cmd [intro]:
+  "type_inv_Chan2_Cmd N sk \<Longrightarrow> i \<le> N \<Longrightarrow> type_inv_Chan2_Cmd N (trans1 (act (n_SendReqE1  i)) sk)"
+  unfolding type_inv_Chan2_Cmd_def n_SendReqE1_def by auto
+
+lemma n_SendReqE2_type_inv_Chan2_Cmd [intro]:
+  "type_inv_Chan2_Cmd N sk \<Longrightarrow> i \<le> N \<Longrightarrow> type_inv_Chan2_Cmd N (trans1 (act (n_SendReqE2  i)) sk)"
+  unfolding type_inv_Chan2_Cmd_def n_SendReqE2_def by auto
+
+lemma n_SendReqS_type_inv_Chan2_Cmd [intro]:
+  "type_inv_Chan2_Cmd N sk \<Longrightarrow> i \<le> N \<Longrightarrow> type_inv_Chan2_Cmd N (trans1 (act (n_SendReqS  i)) sk)"
+  unfolding type_inv_Chan2_Cmd_def n_SendReqS_def by auto 
+
+
+lemma inv_Chan2_Cmd' [simp,intro]:
+  assumes "reachableUpTo (set (allInitSpecs N)) (rules2' N) k s"
+  shows "type_inv_Chan2_Cmd N s"
+  apply (rule invIntro[OF _ _ assms])
+  subgoal for s
+    by (auto simp add: type_inv_Chan2_Cmd_def allInitSpecs_def )
+  subgoal for r sk
+    unfolding rules2'_def apply (auto simp add: pair1_def)
+    subgoal unfolding n_RecvGntEs_def  by auto
+    subgoal unfolding n_RecvGntSs_def   by auto
+    subgoal unfolding  n_SendGntEs_def by auto 
+    subgoal unfolding  n_SendGntSs_def by auto  
+    subgoal unfolding   n_RecvInvAck12s_def
+      using n_RecvInvAck12_type_inv_Chan2_Cmd by auto  
+    subgoal
+      using   n_RecvInvAck2s_def by auto
+    subgoal
+      using  n_SendInvAck1s_def by auto  
+    subgoal
+      using n_SendInvAck2s_def by auto 
+    subgoal
+      using  n_SendInv1s_def by auto  
+    subgoal
+      using n_SendInv2s_def by auto 
+    subgoal
+      using  n_RecvReqEs_def by auto  
+    subgoal
+      using n_RecvReqSs_def by auto 
+    subgoal
+      using n_SendReqE1s_def by auto 
+    subgoal
+      using n_SendReqE2s_def by auto  
+    subgoal
+      using n_SendReqSs_def by auto 
+
+    
+    done
+  done
+   
+
+lemma inv_Chan2_Cmd'' [simp,intro]:
+  assumes a: "reachableUpTo fs rs k s"
+  shows "fs =(set (allInitSpecs N))  \<longrightarrow> rs = rules2' N \<longrightarrow> i \<le> N \<longrightarrow> isEnumVal s (Para ''Chan2.Cmd'' i)"
+  using inv_Chan2_Cmd' unfolding type_inv_Chan2_Cmd_def Inv_def GntS_def GntE_def
+  by (metis Empty_def assms getValueType.simps(1) isEnumVal_def typeOf_def)   
+
+
+definition type_inv_Cache_State :: "nat \<Rightarrow> state \<Rightarrow> bool" where
+  "type_inv_Cache_State N s = 
+(\<forall>i. i \<le> N \<longrightarrow> s ((Para ''Cache.State'' i)) = I  \<or> s (Para ''Cache.State'' i) = S \<or>
+  s (Para ''Cache.State'' i) = E)
+ "
+
+lemma n_RecvGntE_type_inv_Cache_State [intro]:
+  "type_inv_Cache_State N sk \<Longrightarrow> i \<le> N \<Longrightarrow> type_inv_Cache_State N (trans1 (act (n_RecvGntE i)) sk)"
+  unfolding type_inv_Cache_State_def n_RecvGntE_def by auto
+
+lemma n_RecvGntS_type_inv_Cache_State [intro]:
+  "type_inv_Cache_State N sk \<Longrightarrow> i \<le> N \<Longrightarrow> type_inv_Cache_State N (trans1 (act (n_RecvGntS i)) sk)"
+  unfolding type_inv_Cache_State_def n_RecvGntS_def by auto
+
+
+lemma n_SendGntE_type_inv_Cache_State [intro]:
+  "type_inv_Cache_State N sk \<Longrightarrow> i \<le> N \<Longrightarrow> type_inv_Cache_State N (trans1 (act (n_SendGntE N i)) sk)"
+  unfolding type_inv_Cache_State_def n_SendGntE_def by auto
+
+lemma n_SendGntS_type_inv_Cache_State [intro]:
+  "type_inv_Cache_State N sk \<Longrightarrow> i \<le> N \<Longrightarrow> type_inv_Cache_State N (trans1 (act (n_SendGntS  i)) sk)"
+  unfolding type_inv_Cache_State_def n_SendGntS_def by auto
+
+lemma n_RecvInvAck12_type_inv_Cache_State [intro]:
+  "type_inv_Cache_State N sk \<Longrightarrow> i \<le> N \<Longrightarrow> 
+  type_inv_Cache_State N 
+  (trans1 (act ( (strengthenRule2  (constrInvByExcl pair1 i N) (n_RecvInvAck1 i)))) sk)"
+  unfolding type_inv_Cache_State_def n_RecvInvAck1_def apply (auto simp add:strengthenRule2.simps )
+  done
+
+lemma n_RecvInvAck2_type_inv_Cache_State [intro]:
+  "type_inv_Cache_State N sk \<Longrightarrow> i \<le> N \<Longrightarrow> 
+  type_inv_Cache_State N 
+  (trans1 (act (  (n_RecvInvAck2 i))) sk)"
+  unfolding type_inv_Cache_State_def n_RecvInvAck2_def apply (auto simp add:strengthenRule2.simps )
+  done
+lemma n_SendInvAck1_type_inv_Cache_State [intro]:
+  "type_inv_Cache_State N sk \<Longrightarrow> i \<le> N \<Longrightarrow> type_inv_Cache_State N (trans1 (act (n_SendInvAck1 i)) sk)"
+  unfolding type_inv_Cache_State_def n_SendInvAck1_def by auto
+
+lemma n_SendInvAck2_type_inv_Cache_State [intro]:
+  "type_inv_Cache_State N sk \<Longrightarrow> i \<le> N \<Longrightarrow> type_inv_Cache_State N (trans1 (act (n_SendInvAck2 i)) sk)"
+  unfolding type_inv_Cache_State_def n_SendInvAck2_def by auto
+
+lemma n_SendInv1_type_inv_Cache_State [intro]:
+  "type_inv_Cache_State N sk \<Longrightarrow> i \<le> N \<Longrightarrow> type_inv_Cache_State N (trans1 (act (n_SendInv1 i)) sk)"
+  unfolding type_inv_Cache_State_def n_SendInv1_def by auto
+
+lemma n_SendInv2_type_inv_Cache_State [intro]:
+  "type_inv_Cache_State N sk \<Longrightarrow> i \<le> N \<Longrightarrow> type_inv_Cache_State N (trans1 (act (n_SendInv2 i)) sk)"
+  unfolding type_inv_Cache_State_def n_SendInv2_def by auto
+
+
+lemma n_RecvReqE_type_inv_Cache_State [intro]:
+  "type_inv_Cache_State N sk \<Longrightarrow> i \<le> N \<Longrightarrow> type_inv_Cache_State N (trans1 (act (n_RecvReqE N i)) sk)"
+  unfolding type_inv_Cache_State_def n_RecvReqE_def by auto 
+
+lemma n_RecvReqS_type_inv_Cache_State [intro]:
+  "type_inv_Cache_State N sk \<Longrightarrow> i \<le> N \<Longrightarrow> type_inv_Cache_State N (trans1 (act (n_RecvReqS N i)) sk)"
+  unfolding type_inv_Cache_State_def n_RecvReqS_def by auto
+
+lemma n_SendReqE1_type_inv_Cache_State [intro]:
+  "type_inv_Cache_State N sk \<Longrightarrow> i \<le> N \<Longrightarrow> type_inv_Cache_State N (trans1 (act (n_SendReqE1  i)) sk)"
+  unfolding type_inv_Cache_State_def n_SendReqE1_def by auto
+
+lemma n_SendReqE2_type_inv_Cache_State [intro]:
+  "type_inv_Cache_State N sk \<Longrightarrow> i \<le> N \<Longrightarrow> type_inv_Cache_State N (trans1 (act (n_SendReqE2  i)) sk)"
+  unfolding type_inv_Cache_State_def n_SendReqE2_def by auto
+
+lemma n_SendReqS_type_inv_Cache_State [intro]:
+  "type_inv_Cache_State N sk \<Longrightarrow> i \<le> N \<Longrightarrow> type_inv_Cache_State N (trans1 (act (n_SendReqS  i)) sk)"
+  unfolding type_inv_Cache_State_def n_SendReqS_def by auto 
+
+
+lemma inv_Cache_State' [simp,intro]:
+  assumes "reachableUpTo (set (allInitSpecs N)) (rules2' N) k s"
+  shows "type_inv_Cache_State N s"
+  apply (rule invIntro[OF _ _ assms])
+  subgoal for s
+    by (auto simp add: type_inv_Cache_State_def allInitSpecs_def )
+  subgoal for r sk
+    unfolding rules2'_def apply (auto simp add: pair1_def)
+    subgoal unfolding n_RecvGntEs_def  by auto
+    subgoal unfolding n_RecvGntSs_def   by auto
+    subgoal unfolding  n_SendGntEs_def by auto 
+    subgoal unfolding  n_SendGntSs_def by auto  
+    subgoal unfolding   n_RecvInvAck12s_def
+      using n_RecvInvAck12_type_inv_Cache_State by auto  
+    subgoal
+      using   n_RecvInvAck2s_def by auto
+    subgoal
+      using  n_SendInvAck1s_def by auto  
+    subgoal
+      using n_SendInvAck2s_def by auto 
+    subgoal
+      using  n_SendInv1s_def by auto  
+    subgoal
+      using n_SendInv2s_def by auto 
+    subgoal
+      using  n_RecvReqEs_def by auto  
+    subgoal
+      using n_RecvReqSs_def by auto 
+    subgoal
+      using n_SendReqE1s_def by auto 
+    subgoal
+      using n_SendReqE2s_def by auto  
+    subgoal
+      using n_SendReqSs_def by auto 
+
+    
+    done
+  done
+   
+
+lemma inv_Cache_State'' [simp,intro]:
+  assumes a: "reachableUpTo fs rs k s"
+  shows "fs =(set (allInitSpecs N))  \<longrightarrow> rs = rules2' N \<longrightarrow> i \<le> N \<longrightarrow> isEnumVal s (Para ''Cache.State'' i)"
+  using inv_Cache_State' unfolding type_inv_Cache_State_def I_def S_def E_def
+  by (metis  assms getValueType.simps(1) isEnumVal_def typeOf_def)   
+
+
+
+
+
+
+ 
+definition type_inv_CurCmd :: "nat \<Rightarrow> state \<Rightarrow> bool" where
+  "type_inv_CurCmd N s = 
+(\<forall>i. i \<le> N \<longrightarrow> s ((Ident ''CurCmd'')) = Empty  \<or> s (Ident ''CurCmd'') = ReqS \<or>
+  s (Ident ''CurCmd'') =  ReqE \<or> s ((Ident ''CurCmd'')) = InvAck  \<or> s (Ident ''CurCmd'') = GntS \<or>
+  s (Ident ''CurCmd'') =   Inv \<or>  s (Ident ''CurCmd'') =  GntE)
+ "
+
+lemma n_RecvGntE_type_inv_CurCmd [intro]:
+  "type_inv_CurCmd N sk \<Longrightarrow> i \<le> N \<Longrightarrow> type_inv_CurCmd N (trans1 (act (n_RecvGntE i)) sk)"
+  unfolding type_inv_CurCmd_def n_RecvGntE_def by auto
+
+lemma n_RecvGntS_type_inv_CurCmd [intro]:
+  "type_inv_CurCmd N sk \<Longrightarrow> i \<le> N \<Longrightarrow> type_inv_CurCmd N (trans1 (act (n_RecvGntS i)) sk)"
+  unfolding type_inv_CurCmd_def n_RecvGntS_def by auto
+
+
+lemma n_SendGntE_type_inv_CurCmd [intro]:
+  "type_inv_CurCmd N sk \<Longrightarrow> i \<le> N \<Longrightarrow> type_inv_CurCmd N (trans1 (act (n_SendGntE N i)) sk)"
+  unfolding type_inv_CurCmd_def n_SendGntE_def by auto
+
+lemma n_SendGntS_type_inv_CurCmd [intro]:
+  "type_inv_CurCmd N sk \<Longrightarrow> i \<le> N \<Longrightarrow> type_inv_CurCmd N (trans1 (act (n_SendGntS  i)) sk)"
+  unfolding type_inv_CurCmd_def n_SendGntS_def by auto
+
+lemma n_RecvInvAck12_type_inv_CurCmd [intro]:
+  "type_inv_CurCmd N sk \<Longrightarrow> i \<le> N \<Longrightarrow> 
+  type_inv_CurCmd N 
+  (trans1 (act ( (strengthenRule2  (constrInvByExcl pair1 i N) (n_RecvInvAck1 i)))) sk)"
+  unfolding type_inv_CurCmd_def n_RecvInvAck1_def apply (auto simp add:strengthenRule2.simps )
+  done
+
+lemma n_RecvInvAck2_type_inv_CurCmd [intro]:
+  "type_inv_CurCmd N sk \<Longrightarrow> i \<le> N \<Longrightarrow> 
+  type_inv_CurCmd N 
+  (trans1 (act (  (n_RecvInvAck2 i))) sk)"
+  unfolding type_inv_CurCmd_def n_RecvInvAck2_def apply (auto simp add:strengthenRule2.simps )
+  done
+lemma n_SendInvAck1_type_inv_CurCmd [intro]:
+  "type_inv_CurCmd N sk \<Longrightarrow> i \<le> N \<Longrightarrow> type_inv_CurCmd N (trans1 (act (n_SendInvAck1 i)) sk)"
+  unfolding type_inv_CurCmd_def n_SendInvAck1_def by auto
+
+lemma n_SendInvAck2_type_inv_CurCmd [intro]:
+  "type_inv_CurCmd N sk \<Longrightarrow> i \<le> N \<Longrightarrow> type_inv_CurCmd N (trans1 (act (n_SendInvAck2 i)) sk)"
+  unfolding type_inv_CurCmd_def n_SendInvAck2_def by auto
+
+lemma n_SendInv1_type_inv_CurCmd [intro]:
+  "type_inv_CurCmd N sk \<Longrightarrow> i \<le> N \<Longrightarrow> type_inv_CurCmd N (trans1 (act (n_SendInv1 i)) sk)"
+  unfolding type_inv_CurCmd_def n_SendInv1_def by auto
+
+lemma n_SendInv2_type_inv_CurCmd [intro]:
+  "type_inv_CurCmd N sk \<Longrightarrow> i \<le> N \<Longrightarrow> type_inv_CurCmd N (trans1 (act (n_SendInv2 i)) sk)"
+  unfolding type_inv_CurCmd_def n_SendInv2_def by auto
+
+
+lemma n_RecvReqE_type_inv_CurCmd [intro]:
+  "type_inv_CurCmd N sk \<Longrightarrow> i \<le> N \<Longrightarrow> type_inv_CurCmd N (trans1 (act (n_RecvReqE N i)) sk)"
+  unfolding type_inv_CurCmd_def n_RecvReqE_def by auto 
+
+lemma n_RecvReqS_type_inv_CurCmd [intro]:
+  "type_inv_CurCmd N sk \<Longrightarrow> i \<le> N \<Longrightarrow> type_inv_CurCmd N (trans1 (act (n_RecvReqS N i)) sk)"
+  unfolding type_inv_CurCmd_def n_RecvReqS_def by auto
+
+lemma n_SendReqE1_type_inv_CurCmd [intro]:
+  "type_inv_CurCmd N sk \<Longrightarrow> i \<le> N \<Longrightarrow> type_inv_CurCmd N (trans1 (act (n_SendReqE1  i)) sk)"
+  unfolding type_inv_CurCmd_def n_SendReqE1_def by auto
+
+lemma n_SendReqE2_type_inv_CurCmd [intro]:
+  "type_inv_CurCmd N sk \<Longrightarrow> i \<le> N \<Longrightarrow> type_inv_CurCmd N (trans1 (act (n_SendReqE2  i)) sk)"
+  unfolding type_inv_CurCmd_def n_SendReqE2_def by auto
+
+lemma n_SendReqS_type_inv_CurCmd [intro]:
+  "type_inv_CurCmd N sk \<Longrightarrow> i \<le> N \<Longrightarrow> type_inv_CurCmd N (trans1 (act (n_SendReqS  i)) sk)"
+  unfolding type_inv_CurCmd_def n_SendReqS_def by auto 
+
+
+lemma inv_CurCmd' [simp,intro]:
+  assumes "reachableUpTo (set (allInitSpecs N)) (rules2' N) k s"
+  shows "type_inv_CurCmd N s"
+  apply (rule invIntro[OF _ _ assms])
+  subgoal for s
+    by (auto simp add: type_inv_CurCmd_def allInitSpecs_def )
+  subgoal for r sk
+    unfolding rules2'_def apply (auto simp add: pair1_def)
+    subgoal unfolding n_RecvGntEs_def  by auto
+    subgoal unfolding n_RecvGntSs_def   by auto
+    subgoal unfolding  n_SendGntEs_def by auto 
+    subgoal unfolding  n_SendGntSs_def by auto  
+    subgoal unfolding   n_RecvInvAck12s_def
+      using n_RecvInvAck12_type_inv_CurCmd by auto  
+    subgoal
+      using   n_RecvInvAck2s_def by auto
+    subgoal
+      using  n_SendInvAck1s_def by auto  
+    subgoal
+      using n_SendInvAck2s_def by auto 
+    subgoal
+      using  n_SendInv1s_def by auto  
+    subgoal
+      using n_SendInv2s_def by auto 
+    subgoal
+      using  n_RecvReqEs_def by auto  
+    subgoal
+      using n_RecvReqSs_def by auto 
+    subgoal
+      using n_SendReqE1s_def by auto 
+    subgoal
+      using n_SendReqE2s_def by auto  
+    subgoal
+      using n_SendReqSs_def by auto 
+
+    
+    done
+  done
+   
+
+lemma inv_CurCmd'' [simp,intro]:
+  assumes a: "reachableUpTo fs rs k s"
+  shows "fs =(set (allInitSpecs N))  \<longrightarrow> rs = rules2' N \<longrightarrow> i \<le> N \<longrightarrow> isEnumVal s (Ident ''CurCmd'')"
+  using inv_CurCmd' unfolding type_inv_CurCmd_def Empty_def ReqS_def
+     ReqE_def Inv_def InvAck_def GntS_def GntE_def
+  by (metis  assms getValueType.simps(1) isEnumVal_def typeOf_def)   
+
+
+
+
+
+
+ 
+definition type_inv_ExGntd :: "nat \<Rightarrow> state \<Rightarrow> bool" where
+  "type_inv_ExGntd N s = 
+(\<forall>i. i \<le> N \<longrightarrow> s ((Ident ''ExGntd'')) = true  \<or> s (Ident ''ExGntd'') = false)
+ "
+
+lemma n_RecvGntE_type_inv_ExGntd [intro]:
+  "type_inv_ExGntd N sk \<Longrightarrow> i \<le> N \<Longrightarrow> type_inv_ExGntd N (trans1 (act (n_RecvGntE i)) sk)"
+  unfolding type_inv_ExGntd_def n_RecvGntE_def by auto
+
+lemma n_RecvGntS_type_inv_ExGntd [intro]:
+  "type_inv_ExGntd N sk \<Longrightarrow> i \<le> N \<Longrightarrow> type_inv_ExGntd N (trans1 (act (n_RecvGntS i)) sk)"
+  unfolding type_inv_ExGntd_def n_RecvGntS_def by auto
+
+
+lemma n_SendGntE_type_inv_ExGntd [intro]:
+  "type_inv_ExGntd N sk \<Longrightarrow> i \<le> N \<Longrightarrow> type_inv_ExGntd N (trans1 (act (n_SendGntE N i)) sk)"
+  unfolding type_inv_ExGntd_def n_SendGntE_def by auto
+
+lemma n_SendGntS_type_inv_ExGntd [intro]:
+  "type_inv_ExGntd N sk \<Longrightarrow> i \<le> N \<Longrightarrow> type_inv_ExGntd N (trans1 (act (n_SendGntS  i)) sk)"
+  unfolding type_inv_ExGntd_def n_SendGntS_def by auto
+
+lemma n_RecvInvAck12_type_inv_ExGntd [intro]:
+  "type_inv_ExGntd N sk \<Longrightarrow> i \<le> N \<Longrightarrow> 
+  type_inv_ExGntd N 
+  (trans1 (act ( (strengthenRule2  (constrInvByExcl pair1 i N) (n_RecvInvAck1 i)))) sk)"
+  unfolding type_inv_ExGntd_def n_RecvInvAck1_def apply (auto simp add:strengthenRule2.simps )
+  done
+
+lemma n_RecvInvAck2_type_inv_ExGntd [intro]:
+  "type_inv_ExGntd N sk \<Longrightarrow> i \<le> N \<Longrightarrow> 
+  type_inv_ExGntd N 
+  (trans1 (act (  (n_RecvInvAck2 i))) sk)"
+  unfolding type_inv_ExGntd_def n_RecvInvAck2_def apply (auto simp add:strengthenRule2.simps )
+  done
+lemma n_SendInvAck1_type_inv_ExGntd [intro]:
+  "type_inv_ExGntd N sk \<Longrightarrow> i \<le> N \<Longrightarrow> type_inv_ExGntd N (trans1 (act (n_SendInvAck1 i)) sk)"
+  unfolding type_inv_ExGntd_def n_SendInvAck1_def by auto
+
+lemma n_SendInvAck2_type_inv_ExGntd [intro]:
+  "type_inv_ExGntd N sk \<Longrightarrow> i \<le> N \<Longrightarrow> type_inv_ExGntd N (trans1 (act (n_SendInvAck2 i)) sk)"
+  unfolding type_inv_ExGntd_def n_SendInvAck2_def by auto
+
+lemma n_SendInv1_type_inv_ExGntd [intro]:
+  "type_inv_ExGntd N sk \<Longrightarrow> i \<le> N \<Longrightarrow> type_inv_ExGntd N (trans1 (act (n_SendInv1 i)) sk)"
+  unfolding type_inv_ExGntd_def n_SendInv1_def by auto
+
+lemma n_SendInv2_type_inv_ExGntd [intro]:
+  "type_inv_ExGntd N sk \<Longrightarrow> i \<le> N \<Longrightarrow> type_inv_ExGntd N (trans1 (act (n_SendInv2 i)) sk)"
+  unfolding type_inv_ExGntd_def n_SendInv2_def by auto
+
+
+lemma n_RecvReqE_type_inv_ExGntd [intro]:
+  "type_inv_ExGntd N sk \<Longrightarrow> i \<le> N \<Longrightarrow> type_inv_ExGntd N (trans1 (act (n_RecvReqE N i)) sk)"
+  unfolding type_inv_ExGntd_def n_RecvReqE_def by auto 
+
+lemma n_RecvReqS_type_inv_ExGntd [intro]:
+  "type_inv_ExGntd N sk \<Longrightarrow> i \<le> N \<Longrightarrow> type_inv_ExGntd N (trans1 (act (n_RecvReqS N i)) sk)"
+  unfolding type_inv_ExGntd_def n_RecvReqS_def by auto
+
+lemma n_SendReqE1_type_inv_ExGntd [intro]:
+  "type_inv_ExGntd N sk \<Longrightarrow> i \<le> N \<Longrightarrow> type_inv_ExGntd N (trans1 (act (n_SendReqE1  i)) sk)"
+  unfolding type_inv_ExGntd_def n_SendReqE1_def by auto
+
+lemma n_SendReqE2_type_inv_ExGntd [intro]:
+  "type_inv_ExGntd N sk \<Longrightarrow> i \<le> N \<Longrightarrow> type_inv_ExGntd N (trans1 (act (n_SendReqE2  i)) sk)"
+  unfolding type_inv_ExGntd_def n_SendReqE2_def by auto
+
+lemma n_SendReqS_type_inv_ExGntd [intro]:
+  "type_inv_ExGntd N sk \<Longrightarrow> i \<le> N \<Longrightarrow> type_inv_ExGntd N (trans1 (act (n_SendReqS  i)) sk)"
+  unfolding type_inv_ExGntd_def n_SendReqS_def by auto 
+
+
+lemma inv_ExGntd' [simp,intro]:
+  assumes "reachableUpTo (set (allInitSpecs N)) (rules2' N) k s"
+  shows "type_inv_ExGntd N s"
+  apply (rule invIntro[OF _ _ assms])
+  subgoal for s
+    by (auto simp add: type_inv_ExGntd_def allInitSpecs_def )
+  subgoal for r sk
+    unfolding rules2'_def apply (auto simp add: pair1_def)
+    subgoal unfolding n_RecvGntEs_def  by auto
+    subgoal unfolding n_RecvGntSs_def   by auto
+    subgoal unfolding  n_SendGntEs_def by auto 
+    subgoal unfolding  n_SendGntSs_def by auto  
+    subgoal unfolding   n_RecvInvAck12s_def
+      using n_RecvInvAck12_type_inv_ExGntd by auto  
+    subgoal
+      using   n_RecvInvAck2s_def by auto
+    subgoal
+      using  n_SendInvAck1s_def by auto  
+    subgoal
+      using n_SendInvAck2s_def by auto 
+    subgoal
+      using  n_SendInv1s_def by auto  
+    subgoal
+      using n_SendInv2s_def by auto 
+    subgoal
+      using  n_RecvReqEs_def by auto  
+    subgoal
+      using n_RecvReqSs_def by auto 
+    subgoal
+      using n_SendReqE1s_def by auto 
+    subgoal
+      using n_SendReqE2s_def by auto  
+    subgoal
+      using n_SendReqSs_def by auto 
+
+    
+    done
+  done
+   
+
+lemma inv_ExGntd'' [simp,intro]:
+  assumes a: "reachableUpTo fs rs k s"
+  shows "fs =(set (allInitSpecs N))  \<longrightarrow> rs = rules2' N \<longrightarrow> i \<le> N \<longrightarrow> isBoolVal s (Ident ''ExGntd'')"
+  using inv_ExGntd' unfolding type_inv_ExGntd_def true_def false_def
+  using assms by fastforce    
+
+
+lemma rule2'IsSym:
+  "symProtRules' N (rules2' N)"
+  unfolding rules2'_def
+  apply (intro symProtRulesUnion)
+  using n_RecvGntEsIsSym apply blast
+  using n_RecvGntSsIsSym apply blast
+  using n_SendGntEsIsSym apply blast
+  using n_SendGntSsIsSym apply blast
+  using n_RecvInvAck12_ref' n_RecvInvAck12s_def symParaRuleInfSymRuleSet wellFormedSendReqE2(1) apply auto[1]
+  using n_RecvInvAck2sIsSym apply blast
+  using n_SendInvAck1sIsSym apply blast
+  using n_SendInvAck2sIsSym apply blast
+  using n_SendInv1sIsSym apply blast
+  using n_SendInv2sIsSym apply blast
+  using n_RecvReqEsIsSym apply blast
+  using n_RecvReqSsIsSym apply blast
+  using n_SendReqE1sIsSym apply blast
+  using n_SendReqE2sIsSym apply blast
+  using n_SendReqSsIsSym by blast
+  
+
+lemma absProtSim:
+  assumes a2: "M < N"
+    and a3: "M = 1"
+    and a4: "\<forall>i f s.
+       f \<in> F \<longrightarrow>
+       reachableUpTo {f'. \<exists>f. f \<in> (set (allInitSpecs N))\<and> f' = absTransfForm M f}
+        (absRules M) i s \<longrightarrow>
+       formEval (constrInv f 0 1) s"
+  shows "\<forall>f s. f \<in> constrInvByExcls F N \<longrightarrow> 
+    reachableUpTo (set (allInitSpecs N)) (rules' N) i s \<longrightarrow> formEval f s"
+proof (rule_tac ?rs2.0="rules2' N" in CMP)
+  show "\<And>r. r \<in> rules' N \<longrightarrow> wellFormedRule N r"
+    apply (auto simp add: rules'_def 
+          n_RecvGntEs_def symRecvGntE(2)
+   n_RecvGntSs_def n_RecvGntS_def  symRecvGntS(2)
+   n_SendGntEs_def n_SendGntE_def symSendGntE(2)
+   n_SendGntSs_def n_SendGntS_def symSendGntS(2)
+   n_RecvInvAck1s_def n_RecvInvAck1_def symRecvInvAck1(2)
+   n_RecvInvAck2s_def n_RecvInvAck2_def symRecvInvAck2(2)
+   n_SendInvAck1s_def n_SendInvAck1_def symSendInvAck1(2)
+   n_SendInvAck2s_def n_SendInvAck2_def symSendInvAck2(2)
+   n_SendInv1s_def n_SendInv1_def symSendInv1(2)
+   n_SendInv2s_def n_SendInv2_def symSendInv2(2)
+   n_RecvReqEs_def n_RecvReqE_def symRecvReqE(2)
+    n_RecvReqSs_def n_RecvReqS_def symRecvReqS(2)
+   n_SendReqE1s_def n_SendReqE1_def symSendReqE1(2)
+   n_SendReqE2s_def n_SendReqE2_def symSendReqE2(2)
+   n_SendReqSs_def n_SendReqS_def symSendReqS(2))
+    by (metis act.simps symRecvGntE(2) wellFormedRule.elims(3))
+next
+  show "\<forall>f. f \<in> F \<longrightarrow> symPair f N"
+    by (auto simp add: F_def pair1_def symParamForm_def)
+next
+  show "symProtRules' N (rules' N)"
+    using rulesSym' by blast
+next
+  show "symPredSet' N (set (allInitSpecs N))"
+  proof -
+    have b1:"(set (allInitSpecs N)) =
+      {(initSpec0 N)} \<union>
+    {(initSpec1 N)}\<union>
+    {(initSpec2 N)}\<union>
+    {(initSpec3 N)}\<union>
+    {(initSpec4 N)}\<union>
+    {(initSpec5 N)}\<union>
+    {initSpec6} \<union>
+    {initSpec7}" (is "?LHS=?RHS")
+      using allInitSpecs_def by auto
+    have b2:"symPredSet' N ?RHS"
+      using symPreds by blast
+    show "symPredSet' N (set (allInitSpecs N))"
+      using b1 b2 by auto  
+  qed    
+next
+  show "M \<le> N"
+    using a2 by auto
+next
+  show "\<forall>s i f. reachableUpTo ((set (allInitSpecs N))) (rules2' N) i s \<longrightarrow>
+        f \<in> F \<longrightarrow> (\<forall>v. v \<in> varOfForm (constrInv f 0 1) \<longrightarrow> s v = abs1 M s v)"
+    apply auto
+    using inv_ExGntd''  inv_CurCmd'' inv_Cache_State'' inv_Chan2_Cmd'' inv_Chan3_Cmd'' 
+      enumValAbsRemainSame boolValAbsRemainSame
+    unfolding F_def pair1_def using a2 a3 apply auto
+    apply (metis absTransfVar.simps(1) less_imp_le varType.distinct(3))
+    by (metis absTransfVar.simps(1) less_imp_le varType.distinct(3))
+next
+  show "\<forall>r'. r' \<in> rules2' N \<longrightarrow>
+         (\<exists>r f i. f \<in> F \<and> r \<in> rules' N \<and> i \<le> N \<and> r' = strengthenRule2 (constrInvByExcl f i N) r) \<or>
+         r' \<in> rules' N"
+  proof -
+    have "\<exists>r f i. f \<in> F \<and> r \<in> rules' N \<and> i \<le> N \<and> r' = strengthenRule2 (constrInvByExcl f i N) r"
+      if "r' \<in> n_RecvInvAck12s N" for r'
+      using that apply (auto simp add: n_RecvInvAck12s_def)
+      subgoal for i
+        apply (rule exI[where x="n_RecvInvAck1   i"])
+        unfolding F_def pair1_def 
+        apply (auto simp add: constrInvByExcl_def strengthenRule2.simps 
+             n_RecvInvAck12s_def n_RecvInvAck1_def rules'_def  )
+        by (simp add: false_def n_RecvInvAck1_def n_RecvInvAck1s_def)
+      done
+    then show ?thesis
+      apply (unfold rules2'_def rules'_def) by auto
+  qed
+next
+  show "symProtRules' N (rules2' N)"
+    using rule2'IsSym by blast 
+next
+  show "\<forall>r. r \<in> rules' N \<longrightarrow>
+    (\<exists>f. f \<in> constrInvByExcls F N \<and> strengthenRule2 f r \<in> rules2' N) \<or> r \<in> rules2' N"
+  proof -
+    have "\<exists>f. f \<in> constrInvByExcls F N \<and> strengthenRule2 f r \<in>
+    rules2' N"
+      if "r \<in> n_RecvInvAck1s N" for r
+      using that apply (auto simp add: n_RecvInvAck1s_def)
+      subgoal for i
+        apply (rule exI[where x="constrInvByExcl pair1 i N"])
+        by (auto simp add: F_def pair1_def constrInvByExcl_def strengthenRule2.simps n_RecvInvAck12s_def)
+      done
+    then show ?thesis
+      apply (unfold rules2'_def rules'_def) by auto
+  qed
+next 
+  show "1 \<le> N"
+    using a2 a3 by arith  
+next 
+  show "\<forall>i f s.
+       f \<in> F \<longrightarrow>
+       reachableUpTo {f'. \<exists>f. f \<in>set (allInitSpecs N) \<and> f' = absTransfForm M f}
+        {r'. \<exists>r. r \<in> rules2' N \<and> r' = absTransfRule M r} i s \<longrightarrow>
+       formEval (constrInv f 0 1) s"
+  proof -
+    have a: "{r'. \<exists>r. r \<in> rules2' N \<and> r' = absTransfRule M r} = absTransfRule M ` (rules2' N)"
+      by auto
+    show ?thesis
+      unfolding a absAll[OF a2]
+      using a2 a3 a4 absAll by auto
+  qed
+qed
+
 end
+
